some more nand

test/monniaux/nand/nand.c
@@ -1,0 +1,3 @@
+unsigned not(unsigned x) {
+  return ~x;
+}
